Metacoq WIP

practice/meta_zulip.v
@@ -1,5 +1,10 @@
 Require Import MetaCoq.Template.All.
 From MetaCoq.Common Require Import config.
+From MetaCoq.Utils Require Import utils.
+From Equations Require Import Equations.
+Require Import MetaCoq.Quotation.ToTemplate.Init.
+
+(* From MetaCoq.PCUIC Require Import PCUICTyping. *)
 Module Test.
 
 Import MCMonadNotation.
@@ -66,7 +71,30 @@ Fixpoint plus2 (n : nat2) (m : nat2) : nat2 :=
 
 
 Definition P : Prop := forall n : nat2, plus2 O n = n.
+Check tProd.
 MetaCoq Quote Recursively Definition P_quoted := P.
+
+Lemma something :  (forall n : nat2, plus2 O n = n) = P.
+Proof.
+  unfold P.
+  exact eq_refl.
+Qed.
+
+Print something.
+
+MetaCoq Quote Recursively Definition sth_q := something.
+Print sth_q.
+
+Lemma P_act: P.
+Proof.
+unfold P.
+reflexivity.
+Qed.
+
+Print P_act.
+
+MetaCoq Quote Recursively Definition t_quoted := P_act.
+Print t_quoted.
 
 MetaCoq Quote Recursively Definition nat_quoted := nat2.
 Definition ind_decls := InductiveDecl nat_inductive.
@@ -74,22 +102,108 @@ Definition ind_decls := InductiveDecl nat_inductive.
 Definition kername_of_string (s : string) : kername :=
   (MPfile [], s).
 
+
 Definition global_declaraton_nat := (kername_of_string "some", ind_decls). 
-Definition Sigma_env: global_env  := add_global_decl (fst P_quoted) global_declaraton_nat.
+Definition Sigma_env: global_env  := add_global_decl (fst sth_q) global_declaraton_nat.
 Definition universes := Monomorphic_ctx.
 
 Definition Sigma : global_env_ext := (Sigma_env, universes).
-
+Search typing.
 Local Existing Instance default_checker_flags.
 
+Locate ">>=".
 
 Check tmUnquote.
+Compute tmUnquote P_quoted.2.
+MetaCoq Run (tmMkDefinition "sts"%bs P_quoted.2).
+Print sts.
+Compute P_quoted.2.
+Compute tmMkInductive' nat_inductive.
+
+Definition P_copy :=
+  (tProd
+  {|
+    binder_name := nNamed "n"; binder_relevance := Relevant
+  |}
+  (tInd
+     {|
+       inductive_mind :=
+         (MPdot (MPfile ["meta_zulip"]) "Test", "nat2");
+       inductive_ind := 0
+     |} [])
+  (tApp
+     (tInd
+        {|
+          inductive_mind :=
+            (MPfile ["Logic"; "Init"; "Coq"], "eq");
+          inductive_ind := 0
+        |} [])
+     [tInd
+        {|
+          inductive_mind :=
+            (MPdot (MPfile ["meta_zulip"]) "Test", "nat2");
+          inductive_ind := 0
+        |} [];
+      tApp
+        (tConst
+           (MPdot (MPfile ["meta_zulip"]) "Test", "plus2") [])
+        [tConstruct
+           {|
+             inductive_mind :=
+               (MPdot (MPfile ["meta_zulip"]) "Test", "nat2");
+             inductive_ind := 0
+           |} 0 []; tRel 0]; tRel 0])).
+
+Check P_copy.
+
+MetaCoq Unquote Definition P_copyun := P_copy.
+Print P_copyun.
+MetaCoq Run (tmMkDefinition "P2" P_quoted.2).
+Print P2.
+Print P_quoted.
+Print nat.
+Print plus.
+Print Init.Nat.add.
+
+Check tApp.
+
+(* Definition Sigma2_env:= empty_global_env.
+Definition Sigma2 : global_env_ext := (Sigma2_env, universes). *)
+
+
+Class Add (T:Type) := {
+  zero: T;
+  plus: T -> T -> T
+}.
+
+Lemma P1 (T:Type) (H: Add T) (n:T) : plus zero n = n.
+
+
 
 Lemma XYZ : 
-  {t & Sigma ;;; [ ] |- t : tApp P_quoted.2 (snd nat_quoted::nil) }.
+  {t & Sigma ;;; [ ] |- t : P_quoted.2 }.
   Proof.
-  unfold P_quoted. 
+    simpl.
+    eexists.
+    (* unfold Sigma. unfold Sigma_env.
+    unfold add_global_decl. *)
+    simpl.
+    eapply (refine_type).
+    2: { unfold P_copy.
+    simpl.
+    
+    replace_quotation_of_goal ().
+    }
+    
 
+ Check squash.
+ Locate squash.
+  Lemma XYZ : 
+  {t |  Sigma ;;; [ ] |- t : tApp P_quoted.2 (snd nat_quoted::nil) }.
+  Proof.
+
+Lemma XYZ : 
+  {t & Sigma ;;; [ ] |- t :  }.
 
 
 Lemma XYZ : 
