practice/metaprac2.v
@@ -4,13 +4,133 @@ Require Import MetaCoq.Template.All.
 Module monad.
 
 Import MCMonadNotation.
+Import List.
 From MetaCoq Require Import bytestring.
 Import String.
 Open Scope bs.
 
+Check tmDefinition.
+Check tmMkDefinition.
+Check tmMkInductive'.
+
 MetaCoq Run (tmDefinition "foo" 24). (*Definition foo := 24.*)
 
-Print foo.
+MetaCoq Run (tmDefinition "foo2" <% 1 %>).
+Check tmMkInductive'.
+
+MetaCoq Quote Recursively Definition quotednat := nat.
+Print quotednat.
+
+Definition nat_inductive :=
+  {|
+  ind_finite := Finite;
+  ind_npars := 0;
+  ind_params := [];
+  ind_bodies :=
+    [{|
+       ind_name := "nat2";
+       ind_indices := [];
+       ind_sort := sType (Universe.make' Level.lzero);
+       ind_type := tSort (sType (Universe.make' Level.lzero));
+       ind_kelim := IntoAny;
+       ind_ctors :=
+         [{|
+            cstr_name := "O";
+            cstr_args := [];
+            cstr_indices := [];
+            cstr_type := tRel 0;
+            cstr_arity := 0
+          |};
+          {|
+            cstr_name := "S";
+            cstr_args :=
+              [{|
+                 decl_name :=
+                   {|
+                     binder_name := nAnon;
+                     binder_relevance := Relevant
+                   |};
+                 decl_body := None;
+                 decl_type := tRel 0
+               |}];
+            cstr_indices := [];
+            cstr_type :=
+              tProd
+                {|
+                  binder_name := nAnon; binder_relevance := Relevant
+                |} (tRel 0) (tRel 1);
+            cstr_arity := 1
+          |}];
+       ind_projs := [];
+       ind_relevance := Relevant
+     |}];
+  ind_universes := Monomorphic_ctx;
+  ind_variance := None
+|}.
+
+MetaCoq Run (tmMkInductive' nat_inductive).
+Print nat2.
+
+Fixpoint plus2 (n : nat2) (m : nat2) : nat2 :=
+  match n with
+  | O => m
+  | S n' => S (plus2 n' m)
+  end.
+
+
+Definition P : Prop := forall n : nat2, plus2 O n = n.
+MetaCoq Quote Recursively Definition nat_quoted := nat2.
+Compute fst nat_quoted.
+
+MetaCoq Quote Recursively Definition P_quoted := P.
+Print P_quoted.
+Check P_quoted.
+Compute snd P_quoted.
+Compute fst P_quoted.
+Check empty_global_env.
+Check add_global_decl.
+Definition ind_decls := InductiveDecl nat_inductive.
+Locate "×".
+(* Definition ind_global_env:=add_global_decl empty_global_env (prod ind_decls nat2).  *)
+Check Monomorphic_ctx.
+Locate "::".
+Locate "*".
+
+Definition kername_of_string (s : string) : kername :=
+  (MPfile [], s).
+
+Definition global_declaraton_nat := (kername_of_string "some", ind_decls). 
+Definition Sigma_env: global_env  := add_global_decl (fst P_quoted) global_declaraton_nat.
+Definition universes := Monomorphic_ctx.
+Print prod.
+Locate "*".
+
+Definition Sigma : global_env_ext := (Sigma_env, universes).
+Locate "*".
+Print prod.
+Check InductiveDecl.
+Check Sigma_env.
+
+Check tApp.
+Check exist.
+(* Definition XYZ : forall n, exists t, Sigma ;;; [ ] |- t : tApp <% P %> (snd nat_quoted::nil). *)
+Lemma XYZ : 
+  {t | Sigma ;;; [ ] |- t : tApp <% P %> (snd nat_quoted::nil) }.
+  
+  Lemma XYZ : 
+  {t | (isType Sigma [ ] t) (tApp <% P %> (snd nat_quoted::nil)) }.
+  
+
+
+
+
+Definition nat_term := <% nat %>.
+Print nat_term.
+MetaCoq Run (tmMkInductive' <% nat %>).
+Check nat.
+
+Compute <% 1 %>.
+Print foo2.
 
 MetaCoq Test Quote (fun x : nat => x).
 
